More event for leaf signature predicate

fstar/MLS.TreeSync.Symbolic.LeafNodeSignature.fst
@@ -72,8 +72,13 @@ let tree_has_event_arithmetic_lemma l i =
   )
 #pop-options
 
-val tree_has_event: tkt:treekem_types dy_bytes -> principal -> timestamp -> mls_bytes dy_bytes -> (l:nat & i:tree_index l & treesync dy_bytes tkt l i) -> prop
-let tree_has_event tkt prin time group_id (|l, i, t|) =
+val leaf_node_has_event: #tkt:treekem_types dy_bytes -> principal -> timestamp -> leaf_node_tbs_nt dy_bytes tkt -> prop
+let leaf_node_has_event #tkt prin time ln_tbs =
+  let evt_bytes = serialize _ ln_tbs in
+  did_event_occur_before time prin ("MLS.TreeSync.LeafNodeEvent", [evt_bytes])
+
+val tree_has_event: #tkt:treekem_types dy_bytes -> principal -> timestamp -> mls_bytes dy_bytes -> (l:nat & i:tree_index l & treesync dy_bytes tkt l i) -> prop
+let tree_has_event #tkt prin time group_id (|l, i, t|) =
   tree_has_event_arithmetic_lemma l i;
   let evt: group_has_tree_event dy_bytes tkt = {
     group_id;
@@ -86,11 +91,11 @@ let tree_has_event tkt prin time group_id (|l, i, t|) =
 
 val tree_has_equivalent_event: #l:nat -> #i:tree_index l -> tkt:treekem_types dy_bytes -> principal -> timestamp -> mls_bytes dy_bytes -> treesync dy_bytes tkt l i -> leaf_index l i -> prop
 let tree_has_equivalent_event #l #i tkt prin time group_id t li =
-  (exists (t':treesync dy_bytes tkt l i). equivalent t t' li /\ tree_has_event tkt prin time group_id (|l, i, t'|))
+  (exists (t':treesync dy_bytes tkt l i). equivalent t t' li /\ tree_has_event prin time group_id (|l, i, t'|))
 
-val tree_list_has_pred: tkt:treekem_types dy_bytes -> timestamp -> principal -> mls_bytes dy_bytes -> tree_list dy_bytes tkt -> prop
-let tree_list_has_pred tkt time prin group_id tl =
-  for_allP (tree_has_event tkt prin time group_id) tl
+val tree_list_has_pred: #tkt:treekem_types dy_bytes -> timestamp -> principal -> mls_bytes dy_bytes -> tree_list dy_bytes tkt -> prop
+let tree_list_has_pred #tkt time prin group_id tl =
+  for_allP (tree_has_event prin time group_id) tl
 
 val leaf_node_label: string
 let leaf_node_label = "LeafNodeTBS"
@@ -100,22 +105,23 @@ let leaf_node_spred ku tkt usg time vk ln_tbs_bytes =
   match (parse (leaf_node_tbs_nt dy_bytes tkt) ln_tbs_bytes) with
   | None -> False
   | Some ln_tbs -> (
-    match ln_tbs.data.source with
-    | LNS_commit () -> (
-      exists prin tl.
-        get_signkey_label ku vk == readers [p_id prin] /\
-        tree_list_starts_with_tbs tl ln_tbs_bytes /\
-        tree_list_is_parent_hash_linkedP tl /\
-        tree_list_ends_at_root tl /\
-        tree_list_has_pred tkt time prin ln_tbs.group_id tl
-    )
-    | LNS_update () ->
-      (exists prin.
-        get_signkey_label ku vk == readers [p_id prin] /\
-        tree_has_event tkt prin time ln_tbs.group_id (|0, ln_tbs.leaf_index, TLeaf (Some ({data = ln_tbs.data; signature = empty #dy_bytes;} <: leaf_node_nt dy_bytes tkt))|)
+    exists prin.
+      leaf_node_has_event prin time ln_tbs /\ (
+      match ln_tbs.data.source with
+      | LNS_commit () -> (
+        exists (tl: tree_list dy_bytes tkt).
+          get_signkey_label ku vk == readers [p_id prin] /\
+          tree_list_starts_with_tbs tl ln_tbs_bytes /\
+          tree_list_is_parent_hash_linkedP tl /\
+          tree_list_ends_at_root tl /\
+          tree_list_has_pred time prin ln_tbs.group_id tl
       )
-    | LNS_key_package () ->
-      True //forall li. tkp.pred time (|0, li, TLeaf (Some ({data = ln_tbs.data; signature = empty #dy_bytes;} <: leaf_node_nt dy_bytes tkp.types))|)
+      | LNS_update () -> (
+        get_signkey_label ku vk == readers [p_id prin] /\
+        tree_has_event prin time ln_tbs.group_id (|0, ln_tbs.leaf_index, TLeaf (Some ({data = ln_tbs.data; signature = empty #dy_bytes;} <: leaf_node_nt dy_bytes tkt))|)
+      )
+      | LNS_key_package () -> True
+      )
   )
 
 val has_leaf_node_tbs_invariant: treekem_types dy_bytes -> global_usage -> prop
@@ -272,17 +278,17 @@ let parent_hash_implies_event #l #i gu time tkt group_id t ast =
         tree_list_starts_with_tbs leaf_tl ln_tbs_bytes /\
         tree_list_is_parent_hash_linkedP leaf_tl /\
         tree_list_ends_at_root leaf_tl /\
-        tree_list_has_pred tkt time_sig prin ln_tbs.group_id leaf_tl
+        tree_list_has_pred time_sig prin ln_tbs.group_id leaf_tl
       returns tree_has_equivalent_event tkt authentifier time group_id t authentifier_li
       with _. (
         let (b1, b2) = parent_hash_guarantee_theorem my_tl leaf_tl ln_tbs_bytes in
         hash_hash_inj b1 b2;
         last_tree_equivalent my_tl leaf_tl leaf_i;
-        for_allP_eq (tree_has_event tkt prin time_sig group_id) leaf_tl;
+        for_allP_eq (tree_has_event prin time_sig group_id) leaf_tl;
         is_verification_key_to_signkey_label gu "MLS.LeafSignKey" (readers [p_id authentifier]) time ln.data.signature_key;
         readers_is_injective prin authentifier;
         let (|_, _, original_t|) = List.Tot.index leaf_tl (List.Tot.length my_tl - 1) in
-        introduce exists (t':treesync dy_bytes tkt l i). equivalent t t' authentifier_li /\ tree_has_event tkt authentifier time group_id (|l, i, t'|)
+        introduce exists (t':treesync dy_bytes tkt l i). equivalent t t' authentifier_li /\ tree_has_event authentifier time group_id (|l, i, t'|)
         with original_t
         and ()
       )
@@ -394,9 +400,11 @@ val external_path_has_pred: #tkt:treekem_types dy_bytes -> #l:nat -> #li:leaf_in
   (ensures fun _ -> True)
 let external_path_has_pred #tkt #l #li prin time t p group_id =
   let auth_p = external_path_to_path_nosig t p group_id in
+  let auth_ln = get_path_leaf auth_p in
   path_is_parent_hash_valid_external_path_to_path_nosig t p group_id;
   path_is_filter_valid_external_path_to_path_nosig t p group_id;
-  tree_list_has_pred tkt time prin group_id (path_to_tree_list t auth_p)
+  leaf_node_has_event prin time ({data = auth_ln.data; group_id; leaf_index = li;}) /\
+  tree_list_has_pred time prin group_id (path_to_tree_list t auth_p)
 
 #push-options "--z3rlimit 50"
 val is_valid_external_path_to_path: #tkt:treekem_types dy_bytes -> #l:nat -> #li:leaf_index l 0 -> gu:global_usage -> prin:principal -> time:timestamp -> t:treesync dy_bytes tkt l 0 -> p:external_pathsync dy_bytes tkt l 0 li -> group_id:mls_bytes dy_bytes -> sk:sign_private_key dy_bytes -> nonce:sign_nonce dy_bytes -> Lemma
@@ -437,7 +445,8 @@ let is_valid_external_path_to_path #tkt #l #li gu prin time t p group_id sk nonc
     tree_list_starts_with_tbs tl new_ln_tbs_bytes /\
     tree_list_is_parent_hash_linkedP tl /\
     tree_list_ends_at_root tl /\
-    tree_list_has_pred tkt time prin new_ln_tbs.group_id tl
+    tree_list_has_pred time prin new_ln_tbs.group_id tl /\
+    leaf_node_has_event prin time new_ln_tbs
   with prin tl and (
     LabeledCryptoAPI.vk_lemma #gu #time #(readers [p_id prin]) sk
   );
